proof/theories/Example_Ruleset.v
@@ -105,7 +105,7 @@ Definition fw_env : env :=
      e_routes := []; e_rt := fun _ => [];
      e_ifaddr := (fun _ => []); e_ifaddr6 := (fun _ => []);
      e_limit := fun _ => 0; e_quota := fun _ => 0; e_connlimit := fun _ => 0;
-     e_ct := fun _ _ => [] |}.
+     e_ct := fun _ _ => []; e_nat := fun _ => None |}.
 
 (** ** The chains, translated rule-for-rule from ruleset.nft. *)
 
