proof/theories/Optiplex_Gen.v
@@ -39,7 +39,7 @@ Definition base_env : env :=
      e_routes := []; e_rt := fun _ => [];
      e_ifaddr := (fun _ => []); e_ifaddr6 := (fun _ => []);
      e_limit := fun _ => 0; e_quota := fun _ => 0; e_connlimit := fun _ => 0;
-     e_ct := fun _ _ => [] |}.
+     e_ct := fun _ _ => []; e_nat := fun _ => None |}.
 
 Definition gen_env : env := env_with_sets base_env decls.
 
