proof/theories/Payload_Break.v
@@ -34,7 +34,7 @@ Definition empty_env : env :=
   {| e_set := fun _ => []; e_vmap := fun _ => []; e_map := fun _ => [];
      e_routes := []; e_rt := fun _ => []; e_ifaddr := fun _ => []; e_ifaddr6 := fun _ => [];
      e_limit := fun _ => 0; e_quota := fun _ => 0; e_connlimit := fun _ => 0;
-     e_ct := fun _ _ => [] |}.
+     e_ct := fun _ _ => []; e_nat := fun _ => None |}.
 
 Definition bad_pkt : packet :=
   {| pkt_env := empty_env;
