proof/theories/Tcpflag.v
@@ -39,7 +39,7 @@ Definition e0 : env :=
   {| e_set := fun _ => []; e_vmap := fun _ => []; e_map := fun _ => [];
      e_routes := []; e_rt := fun _ => []; e_limit := fun _ => 0;
      e_quota := fun _ => 0; e_ifaddr := fun _ => []; e_ifaddr6 := fun _ => []; e_connlimit := fun _ => 0;
-     e_ct := fun _ _ => [] |}.
+     e_ct := fun _ _ => []; e_nat := fun _ => None |}.
 
 (* A TCP packet whose flags byte (transport header + 13) is [fl].
    FTcpFlags = LPayload PTransport 13 1 reads pkt_th at offset 13, length 1. *)
